(Some) progress on untyped arithmetic

Tapl/Preliminaries.lean
@@ -1,6 +1,9 @@
 /-
 # Mathematical Preleminaries
 -/
+
+import Mathlib.Init.Set
+
 import Mathlib.Data.Nat.Basic
 import Mathlib.Data.Finset.Basic
 import Mathlib.Data.Finset.Card
@@ -11,15 +14,85 @@ namespace «Tapl»
   ## Sets, Relations, and Functions
   -/
 
+  /- 2.1.7 -/
+  def domain {y: β} (R: α → β → Prop): Set α := { x | R x y }
+  def range {x: α} (R: α → β → Prop): Set β := { y | R x y }
+
+  /- 2.1.8 -/
+  def partialFunction (R: α → β → Prop): Prop := ∀ x: α, ∀ y₁ y₂: β, R x y₁ → R x y₂ → y₁ = y₂
+  -- def totalFunction (R: α → β → Prop): Prop := ∀ a: α, partialFunction R ∧ a ∈ domain R
+
+  /- 2.1.9 -/
+  -- def defined (R: α → β → Prop): Prop := ∀ a: α, a ∈ domain R
+
+  /- 2.1.10 -/
+  def preserves (P: α → Prop) (R: α → α → Prop): Prop := ∀ x₁ x₂: α, P x₁ → R x₁ x₂ → P x₂
 
   /-
-  ## Reflexive, Transitive Closure
+  ## Ordered Sets
   -/
 
+  /- 2.2.1 -/
+  def reflexive (R: α → α → Prop): Prop := ∀ x: α, R x x
+  def symmetric (R: α → α → Prop): Prop := ∀ x₁ x₂: α, R x₁ x₂ → R x₂ x₁
+  def transitive (R: α → α → Prop): Prop := ∀ x₁ x₂ x₃: α, R x₁ x₂ → R x₂ x₃ → R x₁ x₃
+  def antisymmetric (R: α → α → Prop): Prop := ∀ x₁ x₂: α, R x₁ x₂ → R x₂ x₁ → x₁ = x₂
+
+  /- 2.2.2 -/
+  def preorder (R: α → α → Prop): Prop := reflexive R ∧ transitive R
+
+  /- 2.2.2 -/
+  def partialOrder (R: α → α → Prop): Prop := preorder R ∧ antisymmetric R
+
+  /- 2.2.3 -/
+
+
+  /- 2.2.4 -/
+  def equivalence (R: α → α → Prop): Prop := reflexive R ∧ transitive R ∧ symmetric R
+
+  /- 2.2.5 -/
+  inductive RC (R: α → α → Prop): α → α → Prop where
+    | base (x₁ x₂: α): R x₁ x₂ → RC R x₁ x₂
+    | refl (x: α): RC R x x
+
+  /- 2.2.5 -/
+  inductive TC (R: α → α → Prop): α → α → Prop where
+    | base (x₁ x₂: α): R x₁ x₂ → TC R x₁ x₂
+    | trans (x₁ x₂ x₃: α): TC R x₁ x₂ → TC R x₂ x₃ → TC R x₁ x₃
+
+  /- 2.2.5 -/
   inductive RTC (R: α → α → Prop): α → α → Prop where
-    | base: ∀ x₁ x₂: α, R x₁ x₂ → RTC R x₁ x₂
-    | refl: ∀ x: α, R x x → RTC R x x
-    | trans: ∀ x₁ x₂ x₃: α, RTC R x₁ x₂ → RTC R x₂ x₃ → RTC R x₁ x₃
+    | base (x₁ x₂: α): R x₁ x₂ → RTC R x₁ x₂
+    | refl (x: α): R x x → RTC R x x
+    | trans (x₁ x₂ x₃: α): RTC R x₁ x₂ → RTC R x₂ x₃ → RTC R x₁ x₃
+
+  /- 2.2.6 -/
+
+  /- 2.2.7 -/
+
+  /- 2.2.8 -/
+
+  /- 2.2.9 -/
+
+  /- 2.2.10 -/
+
+  /-
+  ## Sequences
+  -/
+
+  /- 2.3.1 -/
+
+  /-
+  ## Induction
+  -/
+
+  /- 2.4.1 -/
+
+  /- 2.4.2 -/
+
+  /- 2.4.3 -/
+
+  /- 2.4.4 -/
 
   /-
   ## Deterministic Relations
