Tapl/TyArith.lean
@@ -88,60 +88,162 @@ namespace «Tapl».«TyArith»
     | zero: TypeOf Term.zero .nat
     | pred (n: Term .nat): TypeOf n.pred .nat
     | succ (n: Term .nat): TypeOf n.succ .nat
-    | isZero (n: Term .nat): TypeOf n .nat → TypeOf n.isZero .nat
-    | ite (c: Term .bool) (t f: Term α): TypeOf (.ite c t f) α
+    | isZero (n: Term .nat): TypeOf n.isZero .nat
+    | ite (c: Term .bool) {t f: Term α}: TypeOf (.ite c t f) α
 
   inductive Numeric: Term .nat → Prop where
     | zero: Numeric .zero
-    | succ: Numeric nv → Numeric nv.succ
+    | succ (t: Term .nat) (h: Numeric t): Numeric t.succ
 
   inductive Value: Term α → Prop where
-    | numeric: Numeric nv → Value nv
+    | numeric (t: Term .nat) (h: Numeric t): Value t
     | true: Value .true
     | false: Value .false
 
   inductive Eval₁: Term α → Term α → Prop where
-    | iteTrue: ∀ t f: Term α, Eval₁ (.ite .true t f) t
-    | iteFalse: ∀ t f: Term α, Eval₁ (.ite .false t f) f
-    | ite: ∀ c₁ c₂: Term .bool, ∀ t f: Term α, Eval₁ c₁ c₂ → Eval₁ (.ite c₁ t f) (.ite c₂ t f)
-    | succ: ∀ t₁ t₂: Term .nat, Eval₁ t₁ t₂ → Eval₁ t₁.succ t₂.succ
+    | iteTrue (α: Ty) (t f: Term α): Eval₁ (.ite .true t f) t
+    | iteFalse (α: Ty) (t f: Term α): Eval₁ (.ite .false t f) f
+    | ite (α: Ty) (c₁ c₂: Term .bool) (t f: Term α) (h: Eval₁ c₁ c₂): Eval₁ (.ite c₁ t f) (.ite c₂ t f)
+    | succ (t₁ t₂: Term .nat) (h: Eval₁ t₁ t₂): Eval₁ t₁.succ t₂.succ
     | predZero: Eval₁ Term.zero.pred .zero
-    | predSucc: ∀ t: Term .nat, Numeric t → Eval₁ t.succ.pred t
-    | pred: ∀ t₁ t₂: Term .nat, Eval₁ t₁ t₂ → Eval₁ t₁.pred t₂.pred
+    | predSucc (t: Term .nat) (h: Numeric t): Eval₁ t.succ.pred t
+    | pred (t₁ t₂: Term .nat) (h: Eval₁ t₁ t₂): Eval₁ t₁.pred t₂.pred
     | isZeroZero: Eval₁ Term.zero.isZero .true
-    | isZeroSucc: ∀ t: Term .nat, Numeric t → Eval₁ t.succ.isZero .false
-    | isZero: ∀ t₁ t₂: Term .nat, Eval₁ t₁ t₂ → Eval₁ t₁isZero t₂.isZero
+    | isZeroSucc (t: Term .nat) (h: Numeric t): Eval₁ t.succ.isZero .false
+    | isZero (t₁ t₂: Term .nat) (h: Eval₁ t₁ t₂): Eval₁ t₁isZero t₂.isZero
 
   inductive Eval: Term α → Term α → Prop where
-    | iteTrue: ∀ c: Term .bool, ∀ t₁ t₂ f: Term α, Eval c Term.true → Value t₁ → Eval t₁ t₂ → Eval (.ite c t₁ f) t₂
-    | iteFalse: ∀ c: Term .bool, ∀ t f₁ f₂: Term α, Eval c Term.false → Value f₂ → Eval f₁ f₂ → Eval (.ite c t f₁) f₂
-    | succ: ∀ t₁ t₂: Term .nat, Numeric t₂ → Eval t₁ t₂ → Eval t₁.succ t₂.succ
-    | predZero: ∀ t: Term .nat, Eval t Term.zero → Eval t.pred Term.zero
-    | predSucc: ∀ t₁ t₂: Term .nat, Numeric t₂ → Eval t₁ t₂.succ → Eval t₁.pred t₂
-    | isZeroZero: ∀ t₁: Term .nat, Eval t₁ .zero → Eval t₁.isZero .true
-    | isZeroSucc: ∀ t₁ t₂: Term .nat, Numeric t₂ → Eval t₁ t₂.succ → Eval t₁.isZero .false
+    | iteTrue (α: Ty) (c: Term .bool) (t₁ t₂ f: Term α) (h₁: Eval c Term.true) (h₂: Value t₁) (h₃: Eval t₁ t₂): Eval (.ite c t₁ f) t₂
+    | iteFalse (α: Ty) (c: Term .bool) (t f₁ f₂: Term α) (h₁: Eval c Term.false) (h₂: Value f₂) (h₃: Eval f₁ f₂): Eval (.ite c t f₁) f₂
+    | succ (t₁ t₂: Term .nat) (h₁: Numeric t₂) (h₂: Eval t₁ t₂): Eval t₁.succ t₂.succ
+    | predZero (t: Term .nat) (h: Eval t Term.zero): Eval t.pred Term.zero
+    | predSucc (t₁ t₂: Term .nat) (h₁: Numeric t₂) (h₂: Eval t₁ t₂.succ): Eval t₁.pred t₂
+    | isZeroZero (t₁: Term .nat) (h: Eval t₁ .zero): Eval t₁.isZero .true
+    | isZeroSucc (t₁ t₂: Term .nat) (h₁: Numeric t₂) (h₂: Eval t₁ t₂.succ): Eval t₁.isZero .false
 
-  theorem typeOf_typeOf: ∀ t: Term α, TypeOf t α ↔ t.typeOf = α := sorry
+  section Examples
+    def true: Term .bool := Term.true
+    def false: Term .bool := Term.false
+    def zero: Term .nat := Term.zero
+    def one: Term .nat := zero.succ
+    def two: Term .nat := one.succ
 
-  theorem eval₁_eval₁: ∀ t₁ t₂: Term α, Eval₁ t₁ t₂ ↔ t₁.eval₁ = t₂ := sorry
+    section eval₁
+      example: true.eval₁ = true := rfl
+      example: false.eval₁ = false := rfl
+      example: zero.eval₁ = zero := rfl
+      example: zero.pred.eval₁ = zero := rfl
+      example: two.pred.eval₁ = one := rfl
+      example: two.pred.pred.eval₁ = one.pred := rfl
+      example: one.eval₁ = one := rfl
+      example: two.eval₁ = two := rfl
+      example: one.pred.succ.eval₁ = one := rfl
+      example: zero.isZero.eval₁ = true := rfl
+      example: one.isZero.eval₁ = false := rfl
+      example: two.isZero.eval₁ = false := rfl
+      example: one.pred.succ.pred.isZero.eval₁ = one.pred.isZero := rfl
+      example: zero.pred.isZero.eval₁ = zero.isZero := rfl
+      example: zero.pred.pred.isZero.eval₁ = zero.pred.isZero := rfl
+      example: (Term.ite true one zero).eval₁ = one := rfl
+      example: (Term.ite false one zero).eval₁ = zero := rfl
+      example: (Term.ite zero.isZero one zero).eval₁ = Term.ite true one zero := rfl
+    end eval₁
 
-  theorem eval_eval: ∀ t₁ t₂: Term α, Eval t₁ t₂ ↔ t₁.eval = t₂.eval := sorry
+    section Numeric
+      theorem one_numeric: Numeric one := Numeric.succ Numeric.zero
+    end Numeric
 
-  theorem eval_rtc_eval₁: ∀ t₁ t₂: Term α , RTC Eval₁ t₁ t₂ ↔ Eval t₁ t₂ := sorry
+    section Eval₁
+      private theorem zero_pred_one: Eval₁ one.pred zero := .predSucc .zero
+      private theorem one_pred_two: Eval₁ two.pred one := .predSucc one_numeric
 
-  theorem ty_uniq (h₁: TypeOf t α) (h₂: TypeOf t β): α = β := by
+      example: Eval₁ true true := sorry
+      example: Eval₁ false false := sorry
+      example: Eval₁ zero zero := sorry
+      example: Eval₁ zero.pred zero := .predZero
+      example: Eval₁ two.pred.pred one.pred := .pred one_pred_two
+      example: Eval₁ one one := sorry
+      example: Eval₁ two two := sorry
+      example: Eval₁ one.pred.succ one := .succ zero_pred_one
+      example: Eval₁ zero.isZero .true := .isZeroZero
+      example: Eval₁ one.isZero .false := .isZeroSucc Numeric.zero
+      example: Eval₁ two.isZero .false := .isZeroSucc one_numeric
+      example: Eval₁ one.pred.succ.pred.isZero one.pred.isZero :=
+        have predSuccNumeric: Numeric one.pred :=
+          have zeroNumeric: Numeric zero := .zero
+          sorry
+        .isZero (.predSucc predSuccNumeric)
+      example: Eval₁ zero.pred.isZero zero.isZero := .isZero .predZero
+      example: Eval₁ zero.pred.pred.isZero zero.pred.isZero := .isZero (.pred .predZero)
+      example: Eval₁ (.ite true one zero) one := .iteTrue
+      example: Eval₁ (.ite false one zero) zero := .iteFalse
+      example: Eval₁ (.ite zero.isZero one zero) (.ite true one zero) := .ite .isZeroZero
+    end Eval₁
+
+    section eval
+      example: true.eval = true := rfl
+      example: false.eval = false := rfl
+      example: zero.eval = zero := rfl
+      example: zero.pred.eval = zero := rfl
+      example: two.pred.eval = one := rfl
+      example: two.pred.pred.eval = zero := rfl
+      example: one.eval = one := rfl
+      example: two.eval = two := rfl
+      example: one.pred.succ.eval = one := rfl
+      example: zero.isZero.eval = true := rfl
+      example: one.isZero.eval = false := rfl
+      example: two.isZero.eval = false := rfl
+      example: one.pred.succ.pred.isZero.eval = true := rfl
+      example: zero.pred.isZero.eval = true := rfl
+      example: zero.pred.pred.isZero.eval = true := rfl
+      example: (Term.ite true one zero).eval = one := rfl
+      example: (Term.ite false one zero).eval = zero := rfl
+      example: (Term.ite zero.isZero one zero).eval = one := rfl
+    end eval
+
+    section Eval
+      example: Eval true true := sorry
+      example: Eval false false := sorry
+      example: Eval zero zero := sorry
+      example: Eval zero.pred zero := sorry -- rfl
+      example: Eval two.pred one := sorry -- rfl
+      example: Eval two.pred.pred zero := sorry -- rfl
+      example: Eval one one := sorry
+      example: Eval two two := sorry
+      example: Eval one.pred.succ one := sorry -- rfl
+      example: Eval zero.isZero true := sorry -- rfl
+      example: Eval one.isZero false := sorry -- rfl
+      example: Eval two.isZero false := sorry -- rfl
+      example: Eval one.pred.succ.pred.isZero true := sorry -- rfl
+      example: Eval zero.pred.isZero true := sorry -- rfl
+      example: Eval zero.pred.pred.isZero true := sorry -- rfl
+      example: Eval (Term.ite true one zero) one := sorry -- rfl
+      example: Eval (Term.ite false one zero) zero := sorry -- rfl
+      example: Eval (Term.ite zero.isZero one zero) one := sorry -- rfl
+    end Eval
+  end Examples
+
+  theorem typeOf_typeOf {α: Ty} {t: Term α}: TypeOf t α ↔ t.typeOf = α := sorry
+
+  theorem eval₁_eval₁ {α: Ty} {t₁ t₂: Term α}: Eval₁ t₁ t₂ ↔ t₁.eval₁ = t₂ := sorry
+
+  theorem eval_eval {α: Ty} {t₁ t₂: Term α}: Eval t₁ t₂ ↔ t₁.eval = t₂.eval := sorry
+
+  theorem eval_rtc_eval₁ {α: Ty} {t₁ t₂: Term α}: RTC Eval₁ t₁ t₂ ↔ Eval t₁ t₂ := sorry
+
+  theorem ty_uniq {α β: Ty} {t: Term α} (h₁: TypeOf t α) (h₂: TypeOf t β): α = β := by
     cases h₁ <;> cases h₂ <;> rfl
 
   theorem ty_deriv_uniq: True := sorry
 
   theorem canonical_forms₁: ∀ t: Term .bool, Value t → t = Term.true ∨ t = Term.false
-    | .true, .true => .inl (rfl)
-    | .false, .false => .inr (rfl)
+    | .true, .true => .inl rfl
+    | .false, .false => .inr rfl
 
   theorem canonical_forms₂: ∀ t: Term .nat, Value t → Numeric t
     | .zero, .numeric nv => nv
     | .succ _, .numeric nv => nv
 
-  theorem TypeOf.progress: ∀ t₁: Term α, TypeOf t₁ α → Value t₁ ∨ ∃ t₂: Term α, Eval₁ t₁ t₂ := sorry
-  theorem TypeOf.preservation: ∀ t₁ t₂: Term α, Eval₁ t₁ t₂ → TypeOf t₂ α := sorry
+  theorem TypeOf.progress {α: Ty}: ∀ t₁: Term α, TypeOf t₁ α → Value t₁ ∨ ∃ t₂: Term α, Eval₁ t₁ t₂ := sorry
+  theorem TypeOf.preservation {α: Ty} {t₁ t₂: Term α}: Eval₁ t₁ t₂ → TypeOf t₂ α := sorry
 end «Tapl».«TyArith»
