Tapl/UntypedArith.lean
@@ -4,41 +4,93 @@
 
 import «Tapl».«Preliminaries»
 
+import Mathlib.Init.Set
 import Mathlib.Data.Finset.Basic
 import Mathlib.Data.Finset.Card
+import Mathlib.Data.Finset.Prod
 
 namespace «Tapl».«UntypedArith»
+  /- 3.2.2 -/
   inductive Term: Type where
     | true: Term
     | false: Term
-    | zero: Term
-    | pred: Term → Term
-    | succ: Term → Term
-    | isZero: Term → Term
-    | ite: Term → Term → Term → Term
+    -- | zero: Term
+    -- | pred: Term → Term
+    -- | succ: Term → Term
+    -- | isZero: Term → Term
+    | ite (c t f: Term): Term
   deriving Repr, DecidableEq
 
+  -- TODO: Fix
+  /- 3.2.3 -/
+  def Term.termsᵢ: Nat → Finset Term
+    | .zero => { Term.true, Term.false /-, Term.zero -/ }
+    | .succ n =>
+      let sn := Term.termsᵢ n
+      let ite: Finset Term := { .ite Term.true Term.true Term.true }
+      sn ∪ ite
+
+  /- 3.2.3 -/
+  def Term.terms: Set Term := ⋃ i, Term.termsᵢ i
+
+  -- TODO: Fix
+  /- Exersise 3.2.4 -/
+  example: (Term.termsᵢ 3).card = 3 := rfl
+
+  /- Exercise 3.2.5 -/
+  theorem Term.termsᵢ.cumulative (i: Nat): Term.termsᵢ i ⊆ Term.termsᵢ i.succ := by
+    induction i with
+      | zero =>
+        unfold Term.termsᵢ
+        simp
+      | succ n ih =>
+        unfold Term.termsᵢ
+        simp
+        intro t h
+        sorry
+
+  /- 3.2.6 -/
+  -- TODO
+
+  /- 3.3.1 -/
   def Term.consts: Term → Finset Term
     | .true =>   { .true }
     | .false => { .false }
-    | .zero => { .zero }
-    | .pred t | .succ t | .isZero t => t.consts
+    -- | .zero => { .zero }
+    -- | .pred t | .succ t | .isZero t => t.consts
     | .ite c t f => c.consts ∪ t.consts ∪ f.consts
 
+  /- 3.3.2 -/
   def Term.size: Term → Nat
-    | .true | .false | .zero => 1
-    | .pred t | .succ t | .isZero t => 1 + t.size
+    | .true | .false => 1 --| .zero => 1
+    -- | .pred t | .succ t | .isZero t => 1 + t.size
     | .ite c t f => 1 + c.size + t.size + f.size
 
-  @[local simp]
+  /- 3.3.2 -/
   def Term.depth: Term → Nat
-    | .true | .false | .zero => 1
-    | .pred t | .succ t | .isZero t => 1 + t.depth
-    | .ite c t f => 1 + Nat.max (Nat.max c.depth t.depth) f.depth
+    | .true | .false => 1 --| .zero => 1
+    -- | .pred t | .succ t | .isZero t => 1 + t.depth
+    | .ite c t f => 1 + (c.depth.max t.depth).max f.depth
+
+  /- 3.3.3 -/
+  example (t: Term): t.consts.card ≤ t.size := by
+    induction t with
+      | true => rfl
+      | false => rfl
+      | ite c t f ihc iht ihf =>
+        -- calc (c.consts ∪ t.consts ∪ f.consts).card
+        --   _ ≤ (c.consts ∪ t.consts).card + f.consts.card    := Finset.card_union_le (c.consts ∪ t.consts) f.consts
+        --   _ = f.consts.card + (c.consts ∪ t.consts).card    := by rw [Nat.add_comm]
+        --   _ ≤ f.consts.card + c.consts.card + t.consts.card := congrArg (Nat.add f.consts.card) (Finset.card_union_le c.consts t.consts)
+        -- have h: c.consts.card + t.consts.card + f.consts.card ≤ c.size + t.size + f.size := sorry
+        -- unfold Term.consts Term.size
+        --
+        -- rw [Finset.card_union_eq sorry, Finset.card_union_eq sorry]
+        sorry
 
   def Term.isNumeric: Term → Bool
-    | .zero => Bool.true
-    | .succ n => n.isNumeric
+    -- | .zero => Bool.true
+    -- | .succ n => n.isNumeric
     | _ => Bool.false
 
   def Term.isValue: Term → Bool
@@ -48,14 +100,15 @@ namespace «Tapl».«UntypedArith»
   def Term.eval₁: Term → Term
     | .true => .true
     | .false => .false
-    | .zero => .zero
-    | .pred .zero => .zero
-    | .pred t => t.eval₁.pred
-    | .succ .zero => Term.zero.succ
-    | .succ t => t.eval₁.succ
-    | .isZero .zero => .true
-    | .isZero (.succ _) => .false
-    | .isZero t => t.eval₁.isZero
+    -- | .zero => .zero
+    -- | .pred .zero => .zero
+    -- | .pred (.succ t) => t
+    -- | .pred t => t.eval₁.pred
+    -- | .succ .zero => Term.zero.succ
+    -- | .succ t => t.eval₁.succ
+    -- | .isZero .zero => .true
+    -- | .isZero (.succ _) => .false
+    -- | .isZero t => t.eval₁.isZero
     | .ite .true t _ => t
     | .ite .false _ f => f
     | .ite c t f => .ite c.eval₁ t f
@@ -63,18 +116,18 @@ namespace «Tapl».«UntypedArith»
   def Term.eval: Term → Term
     | .true => .true
     | .false => false
-    | .zero => .zero
-    | .pred n =>
-      match n.eval with
-        | .zero => .zero
-        | .succ n => n
-        | _ => sorry
-    | .succ n => n.eval.succ
-    | .isZero n =>
-      match n.eval with
-        | .zero => .true
-        | .succ _ => .false
-        | _ => sorry
+    -- | .zero => .zero
+    -- | .pred n =>
+    --   match n.eval with
+    --     | .zero => .zero
+    --     | .succ n => n
+    --     | _ => sorry
+    -- | .succ n => n.eval.succ
+    -- | .isZero n =>
+    --   match n.eval with
+    --     | .zero => .true
+    --     | .succ _ => .false
+    --     | _ => sorry
     | .ite c t f =>
       match c.eval with
         | .true => t.eval
@@ -82,72 +135,160 @@ namespace «Tapl».«UntypedArith»
         | _ => sorry
 
   inductive Numeric: Term → Prop where
-    | zero: Numeric Term.zero
-    | succ: ∀ nv: Term, Numeric nv → Numeric nv.succ
+    -- | zero: Numeric Term.zero
+    -- | succ {t: Term} (h: Numeric t): Numeric t.succ
 
   inductive Value: Term → Prop where
-    | numeric: ∀ nv: Term, Numeric nv → Value nv
+    -- | numeric {t: Term} (h: Numeric t): Value t
     | true: Value Term.true
     | false: Value Term.false
 
+  /- 3.5.3 -/
   inductive Eval₁: Term → Term → Prop where
-    | iteTrue: ∀ t f: Term, Eval₁ (.ite .true t f) t
-    | iteFalse: ∀ t f: Term, Eval₁ (.ite .false t f) f
-    | ite: ∀ c₁ c₂ t f: Term, Eval₁ c₁ c₂ → Eval₁ (.ite c₁ t f) (.ite c₂ t f)
-    | succ: ∀ t₁ t₂: Term, Eval₁ t₁ t₂ → Eval₁ t₁.succ t₂.succ
-    | predZero: Eval₁ Term.zero.pred .zero
-    | predSucc: ∀ t: Term, Numeric t → Eval₁ t.succ.pred t
-    | pred: ∀ t₁ t₂: Term, Eval₁ t₁ t₂ → Eval₁ t₁.pred t₂.pred
-    | isZeroZero: Eval₁ Term.zero.isZero .true
-    | isZeroSucc: ∀ t: Term, Numeric t → Eval₁ t.succ.isZero .false
-    | isZero: ∀ t₁ t₂: Term, Eval₁ t₁ t₂ → Eval₁ t₁isZero t₂.isZero
+    | iteTrue (t f: Term): Eval₁ (.ite .true t f) t
+    | iteFalse (t f: Term): Eval₁ (.ite .false t f) f
+    | ite (c₁ c₂ t f: Term) (h: Eval₁ c₁ c₂): Eval₁ (.ite c₁ t f) (.ite c₂ t f)
+    -- | succ (t₁ t₂: Term) (h: Eval₁ t₁ t₂): Eval₁ t₁.succ t₂.succ
+    -- | predZero: Eval₁ Term.zero.pred .zero
+    -- | predSucc (t: Term) (h: Numeric t): Eval₁ t.succ.pred t
+    -- | pred (t₁ t₂: Term) (h: Eval₁ t₁ t₂): Eval₁ t₁.pred t₂.pred
+    -- | isZeroZero: Eval₁ Term.zero.isZero .true
+    -- | isZeroSucc (t: Term) (h: Numeric t): Eval₁ t.succ.isZero .false
+    -- | isZero (t₁ t₂: Term) (h: Eval₁ t₁ t₂): Eval₁ t₁isZero t₂.isZero
+
+  section
+    /- 3.5.1 -/
+    example: Eval₁ (.ite .true .true (.ite .false .false .false)) .true :=
+      Eval₁.iteTrue .true (.ite .false .false .false)
+
+    /- 3.5.3 -/
+    private def s: Term := .ite .true .false .false
+    private def t: Term := .ite s .true .true
+    private def u: Term := .ite .false .true .true
+
+    example: Eval₁ (.ite t .false .false) (.ite u .false .false) :=
+      .iteTrue .false .false
+        |> .ite s .false .true .true
+        |> .ite t u .false .false
+
+    example: Eval₁ (.ite t .false .false) (.ite u .false .false) := by
+      apply Eval₁.ite
+      · apply Eval₁.ite
+        · apply Eval₁.iteTrue
+  end
+
+  /- 3.5.4 -/
+  theorem Eval₁.deterministic {t₁ t₂ t₃: Term}: Eval₁ t₁ t₂ → Eval₁ t₁ t₃ → t₂ = t₃
+    | .iteTrue .true _, .iteTrue .true _
+    | .iteTrue .false _, .iteTrue .false _
+    | .iteTrue (.ite _ _ _) _, .iteTrue (.ite _ _ _) _
+    | .iteFalse _ .true, .iteFalse _ .true
+    | .iteFalse _ .false, .iteFalse _ .false
+    | .iteFalse _ (.ite _ _ _), .iteFalse _ (.ite _ _ _) => rfl
+    | .ite _ c₁ _ _ hc₁, .ite _ c₂ _ _ hc₂ =>
+      have h: c₁ = c₂ := Eval₁.deterministic hc₁ hc₂
+      by rw [h]
+
+    -- | .succ t₁, .succ t₂ => sorry
+    -- | .succ t₁, h => sorry
+    -- | .predZero, .predZero => rfl
+    -- | .predZero, h => sorry
+    -- | .predSucc hn₁, .predSucc hn₂ => sorry
+    -- | .predSucc hn₁, h => sorry
+    -- | .pred ht₁, .pred ht₂ => sorry
+    -- | .pred ht₁, h => sorry
+    -- | .isZeroZero, .isZeroZero => rfl
+    -- | .isZeroZero, h => sorry
+    -- | .isZeroSucc ht₁, .isZeroSucc ht₂ => sorry
+    -- | .isZeroSucc ht₁, h => sorry
+    -- | .isZero ht₁, .isZero ht₂ => sorry
+    -- | .isZero ht₁, h => sorry
+
+  /- 3.5.4 -/
+  example {t₁ t₂ t₃: Term} (h₁: Eval₁ t₁ t₂) (h₂: Eval₁ t₁ t₃): t₂ = t₃ := by
+    induction h₁ with
+      | iteTrue tru₁ fls₁ =>
+        cases h₂ with
+          | iteTrue tru₂ fls₂ => rfl
+          | ite c₁ c₂ tru₂ fls₂ hc₂ => contradiction
+      | iteFalse =>
+        cases h₂ with
+          | iteFalse tru₂ fls₂ => rfl
+          | ite c₁ c₂ tru₂ fls₂ hc₂ => contradiction
+      | ite c₁ c₂ tru₁ tru₂ hc₁ ih =>
+        cases h₂ with
+          | iteTrue tru₂ fls₂ => contradiction
+          | iteFalse tru₂ fls₂ => contradiction
+          | ite c₃ c₄ tru₂ fls₂ hc₂ => rw [_example hc₁ hc₂]
+      -- | succ ht ih => sorry
+      -- | predZero => sorry
+      -- | predSucc hn => sorry
+      -- | pred ht ih => sorry
+      -- | isZeroZero => sorry
+      -- | isZeroSucc ht => sorry
+      -- | isZero ht ih => sorry
+
+  /- 3.5.6 -/
+  def Term.isNormal₁ (t₁: Term): Prop := ¬ ∃ t₂: Term, Eval₁ t₁ t₂
+
+  /- 3.5.15 -/
+  def Term.stuck₁ (t: Term): Prop := t.isNormal₁ ∧ ¬ Value t
+
+  /- 3.5.7 -/
+  theorem Value.normal₁ {t: Term}: Value t → t.isNormal₁ -- ¬ ∃ t₂: Term, Eval₁ t t₂
+    | .true => sorry
+    | .false => sorry
+
+  example {t: Term} (h: Value t): t.isNormal₁ := by
+    unfold Term.isNormal₁ Not
+    intro h₁
+    cases h with
+      | true =>
+        apply Exists.elim h₁
+        · intro x h₂
+          contradiction
+      | false =>
+        apply Exists.elim h₁
+        · intro x h₂
+          contradiction
 
   inductive Eval: Term → Term → Prop where
-    | iteTrue: ∀ c t₁ t₂ f: Term, Eval c Term.true → Value t₁ → Eval t₁ t₂ → Eval (.ite c t₁ f) t₂
-    | iteFalse: ∀ c t f₁ f₂: Term, Eval c Term.false → Value f₂ → Eval f₁ f₂ → Eval (.ite c t f₁) f₂
-    | succ: ∀ t₁ t₂: Term, Numeric t₂ → Eval t₁ t₂ → Eval t₁.succ t₂.succ
-    | predZero: ∀ t: Term, Eval t Term.zero → Eval t.pred Term.zero
-    | predSucc: ∀ t₁ t₂: Term, Numeric t₂ → Eval t₁ t₂.succ → Eval t₁.pred t₂
-    | isZeroZero: ∀ t₁: Term, Eval t₁ .zero → Eval t₁.isZero .true
-    | isZeroSucc: ∀ t₁ t₂: Term, Numeric t₂ → Eval t₁ t₂.succ → Eval t₁.isZero .false
+    | value (t: Term) (h: Value t): Eval t t
+    | iteTrue (c t₁ t₂ f: Term) (h₁: Eval c Term.true) (h₂: Value t₂) (h₃: Eval t₁ t₂): Eval (.ite c t₁ f) t₂
+    | iteFalse (c t f₁ f₂: Term) (h₁: Eval c Term.false) (h₂: Value f₂) (h₃: Eval f₁ f₂): Eval (.ite c t f₁) f₂
+    -- | succ (t₁ t₂: Term) (h₁: Numeric t₂) (h₂: Eval t₁ t₂): Eval t₁.succ t₂.succ
+    -- | predZero (t: Term) (h: Eval t Term.zero): Eval t.pred Term.zero
+    -- | predSucc (t₁ t₂: Term) (h₁: Numeric t₂) (h₂: Eval t₁ t₂.succ): Eval t₁.pred t₂
+    -- | isZeroZero (t₁: Term) (h: Eval t₁ .zero): Eval t₁.isZero .true
+    -- | isZeroSucc (t₁ t₂: Term) (h₁: Numeric t₂) (h₂: Eval t₁ t₂.succ): Eval t₁.isZero .false
 
-  def Term.isNormal: ∀ t₁: Term, ¬ ∃ t₂: Term, Eval t₁ t₂ := sorry
+  /- 3.5.6 -/
+  def Term.isNormal (t₁: Term): Prop := ¬ ∃ t₂: Term, Eval t₁ t₂
+  /- 3.5.15 -/
+  def Term.stuck (t: Term): Prop := t.isNormal ∧ ¬ Value t
 
-  theorem eval₁_eval₁ (t₁ t₂: Term): Eval₁ t₁ t₂ ↔ t₁.eval₁ = t₂ := sorry
+  /- 3.5.9 -/
+  theorem eval_rtc_eval₁ {t₁ t₂: Term}: RTC Eval₁ t₂ t₂ ↔ Eval t₁ t₂ := sorry
 
-  theorem Eval₁.deterministic (t₁ t₂ t₃: Term): Eval₁ t₁ t₂ → Eval₁ t₁ t₃ → t₂ = t₃
-    | .iteTrue t f, h => sorry
-    | .iteFalse t f, h => sorry
-    | .ite c₁ c₂ t f hc, h => sorry
-    | .succ t₁ t₂ t, h => sorry
-    | .predZero, h => sorry
-    | .predSucc t hn, h => sorry
-    | .pred t₁ t₂ ht, h => sorry
-    | .isZeroZero, h => sorry
-    | .isZeroSucc t ht, h => sorry
-    | .isZero t₁ t₂ ht, h => sorry
+  /- 3.5.11 -/
+  theorem normal_unique {t₁ t₂ t₃: Term} (ht₁: t₂.isNormal) (ht₂: t₂.isNormal): Eval t₁ t₂ → Eval t₂ t₃ → t₂ = t₃
+    | .value .true _, .value .true _ => rfl
+    | .value .false _, .value .false _ => rfl
+    | _, _ => sorry
 
-  example (t₁ t₂ t₃: Term): Eval₁ t₁ t₂ → Eval₁ t₁ t₃ → t₂ = t₃ := by
-    intro h₁₂ h₁₃
-    induction h₁₂ with
-      | iteTrue t f => sorry
-      | iteFalse t f => sorry
-      | ite c₁ c₂ t f hc ih => sorry
-      | succ t₁ t₂ t ih => sorry
-      | predZero => sorry
-      | predSucc t hn => sorry
-      | pred t₁ t₂ ht ih => sorry
-      | isZeroZero => sorry
-      | isZeroSucc t ht => sorry
-      | isZero t₁ t₂ ht ih => sorry
+  example {t₁ t₂ t₃: Term} (ht₁: t₂.isNormal) (ht₂: t₂.isNormal) (he₁: Eval t₁ t₂) (he₂: Eval t₂ t₃): t₂ = t₃ := by
+    induction he₁ with
+      | value tm₁ hv₁ =>
+        cases he₂ with
+          | value tm₂ hv₂ => rfl
+          | iteTrue c tru₁ tru₂ fls h₁ h₂ h₃ => sorry
+          | iteFalse c tru fls₁ fls₂ h₁ h₂ h₃ => sorry
+      | iteTrue => sorry
+      | iteFalse => sorry
 
-  -- theorem Value.normal: ∀ t: Term, Value t → t.isNormal := sorry
+  /- 3.5.12 -/
+  theorem Eval.termination {t₁: Term}: ∃ t₂: Term, t₂.isNormal → Eval t₁ t₂ := sorry
 
-  theorem eval_eval (t₁ t₂: Term): Eval t₁ t₂ ↔ t₁.eval = t₂ := sorry
-
-  theorem eval_rtc_eval₁ (t₁ t₂: Term): RTC Eval₁ t₂ t₂ ↔ Eval t₁ t₂ := sorry
-
-  -- theorem normal_unique (t₁ t₂ t₃: Term): t₂.isNormal → t₂.isNormal → Eval t₁ t₂ → Eval t₂ t₃ → t₂ = t₃ := sorry
-
-  -- theorem Eval.termination (t₁: Term): ∃ t₂: Term, t₂.isNormal ∧ Eval t₁ t₂ := sorry
+  theorem eval₁_eval₁ {t₁ t₂: Term}: Eval₁ t₁ t₂ ↔ t₁.eval₁ = t₂ := sorry
+  theorem eval_eval {t₁ t₂: Term}: Eval t₁ t₂ ↔ t₁.eval = t₂ := sorry
 end «Tapl».«UntypedArith»
