SetTheoryGame/FamilyIntersectionWorld.lean
@@ -2,16 +2,73 @@
 # Family Intersection World
 -/
 
+import Mathlib.Data.Set.Lattice
+
 import «SetTheoryGame».«SubsetWorld»
 import «SetTheoryGame».«ComplementWorld»
 import «SetTheoryGame».«IntersectionWorld»
 import «SetTheoryGame».«UnionWorld»
 
--- theorem fam_inter_def {U: Type} (x: U) (F: Set U → Set (Set U)) : x ∈ ⋂ F ↔ ∀ S ∈ F, x ∈ S := sorry
+theorem fam_inter_def {U: Type} {x: U} {F: Set (Set U)}: x ∈ ⋂₀ F ↔ ∀ S ∈ F, x ∈ S := sorry
+theorem pair_def {U : Type} {S A B: Set U} : S ∈ ({A, B}: Set (Set U)) ↔ S = A ∨ S = B := sorry
 
 /-
 ## Family Intersection is Subset
 -/
 
--- example {A: Set U} {F: Set (Set U)} (h₁: A ∈ F): ⋂₀ F ⊆ A := by
---   sorry
+example {A: Set U} {F: Set (Set U)} (h₁: A ∈ F): ⋂₀ F ⊆ A := by
+  intro x h₂
+  rw [fam_inter_def] at h₂
+  have h₂A: A ∈ F → x ∈ A := h₂ A
+  exact h₂A h₁
+
+/-
+## Intersection of larger family is smaller
+-/
+
+example (F G: Set (Set U)) (h₁: F ⊆ G): ⋂₀ G ⊆ ⋂₀ F := by
+  intro x h₂
+  rw [fam_inter_def]
+  intro y z
+  have h₃: y ∈ G := h₁ z
+  exact h₂ y h₃
+
+/-
+## Intersections of a Pair
+-/
+
+theorem inter_def {U : Type} (x : U) (A B : Set U) : x ∈ A ∩ B ↔ x ∈ A ∧ x ∈ B := sorry
+
+
+
+example (A B: Set U): A ∩ B = ⋂₀ {A, B} := by
+  ext
+  apply Iff.intro
+  · intro h₁
+    rw [fam_inter_def]
+    intro z h₂
+    sorry
+  · intro h₁
+    rw [inter_def]
+    apply And.intro
+    · rw [fam_inter_def] at h₁
+      apply h₁
+      sorry
+    · rw [fam_inter_def] at h₁
+      apply h₁
+
+      sorry
+    -- rw [inter_def]
+
+
+/-
+## Intersection of a Union of Families
+-/
+
+example (F G: Set (Set U)): ⋂₀ (F ∪ G) = (⋂₀ F) ∩ (⋂₀ G) := by
+  ext
+  apply Iff.intro
+  · intro h
+    rw [fam_inter_def] at h
+    sorry
+  · sorry
